src/SimpleTypesNotations.v
@@ -1,17 +1,15 @@
 (** * Notations for Simple Types *)
 
-Set Implicit Arguments.
-
 Require Import SimpleTypes.
 
 Declare Custom Entry DM.
-Notation "[ e ]" := e (e custom DM at level 2).
+Notation "&[ e ]" := e (e custom DM at level 2).
 
-Notation "'a'" := (var 0) (in custom DM at level 0).
-Notation "i" := (var i) (in custom DM at level 0, i ident).
-Notation "tau -> tau'" := (arrow tau tau') (in custom DM at level 1, left associativity).
+Notation "'VA'" := (var 0) (in custom DM at level 0).
+Notation "tau -> tau'" := (arrow tau tau') (in custom DM at level 1, right associativity).
 Notation "( e )" := e (in custom DM, e at level 2).
 
+Notation "{ x }" := x (in custom DM, x constr).
 Notation "x" := x (in custom DM at level 0, x ident).
 
-Check forall tau, [a -> tau] = [a -> tau].
+Check forall tau, &[VA -> tau] = &[VA -> tau].
